fstar_out/BinTree.ml
@@ -1,58 +1,65 @@
 open Prims
-type ('a, 'compare) set =
-  | Node of ('a, unit) set * 'a * Prims.nat * ('a, unit) set 
+let cmp :
+  'a 'b .
+    'a Compare.comparaison -> ('a * 'b) -> ('a * 'b) -> Compare.ordering
+  =
+  fun f ->
+    fun x ->
+      fun y ->
+        f (FStar_Pervasives_Native.fst x) (FStar_Pervasives_Native.fst y)
+type ('a, 'b, 'compare) set =
+  | Node of ('a, 'b, unit) set * ('a * 'b) * Prims.nat * ('a, 'b, unit) set 
   | Leaf 
 let uu___is_Node :
-  'a . 'a Compare.comparaison -> ('a, unit) set -> Prims.bool =
+  'a 'b . 'a Compare.comparaison -> ('a, 'b, unit) set -> Prims.bool =
   fun compare ->
     fun projectee ->
-      match projectee with | Node (left, _1, _2, _3) -> true | uu___ -> false
-let __proj__Node__item__left :
-  'a . 'a Compare.comparaison -> ('a, unit) set -> ('a, unit) set =
+      match projectee with | Node (_0, _1, _2, _3) -> true | uu___ -> false
+let __proj__Node__item___0 :
+  'a 'b . 'a Compare.comparaison -> ('a, 'b, unit) set -> ('a, 'b, unit) set
+  =
   fun compare ->
-    fun projectee -> match projectee with | Node (left, _1, _2, _3) -> left
+    fun projectee -> match projectee with | Node (_0, _1, _2, _3) -> _0
 let __proj__Node__item___1 :
-  'a . 'a Compare.comparaison -> ('a, unit) set -> 'a =
+  'a 'b . 'a Compare.comparaison -> ('a, 'b, unit) set -> ('a * 'b) =
   fun compare ->
-    fun projectee -> match projectee with | Node (left, _1, _2, _3) -> _1
+    fun projectee -> match projectee with | Node (_0, _1, _2, _3) -> _1
 let __proj__Node__item___2 :
-  'a . 'a Compare.comparaison -> ('a, unit) set -> Prims.nat =
+  'a 'b . 'a Compare.comparaison -> ('a, 'b, unit) set -> Prims.nat =
   fun compare ->
-    fun projectee -> match projectee with | Node (left, _1, _2, _3) -> _2
+    fun projectee -> match projectee with | Node (_0, _1, _2, _3) -> _2
 let __proj__Node__item___3 :
-  'a . 'a Compare.comparaison -> ('a, unit) set -> ('a, unit) set =
+  'a 'b . 'a Compare.comparaison -> ('a, 'b, unit) set -> ('a, 'b, unit) set
+  =
   fun compare ->
-    fun projectee -> match projectee with | Node (left, _1, _2, _3) -> _3
+    fun projectee -> match projectee with | Node (_0, _1, _2, _3) -> _3
 let uu___is_Leaf :
-  'a . 'a Compare.comparaison -> ('a, unit) set -> Prims.bool =
+  'a 'b . 'a Compare.comparaison -> ('a, 'b, unit) set -> Prims.bool =
   fun compare ->
     fun projectee -> match projectee with | Leaf -> true | uu___ -> false
-let height : 'a . 'a Compare.comparaison -> ('a, unit) set -> Prims.nat =
+let height :
+  'a 'b . 'a Compare.comparaison -> ('a, 'b, unit) set -> Prims.nat =
   fun f ->
     fun s -> match s with | Node (l, k, s1, r) -> s1 | Leaf -> Prims.int_zero
-let key : 'a . 'a Compare.comparaison -> ('a, unit) set -> 'a =
+let key : 'a 'b . 'a Compare.comparaison -> ('a, 'b, unit) set -> ('a * 'b) =
   fun f -> fun s -> match s with | Node (uu___, k, uu___1, uu___2) -> k
-let left : 'a . 'a Compare.comparaison -> ('a, unit) set -> ('a, unit) set =
+let left :
+  'a 'b . 'a Compare.comparaison -> ('a, 'b, unit) set -> ('a, 'b, unit) set
+  =
   fun f ->
     fun input -> match input with | Node (l, uu___, uu___1, uu___2) -> l
-let right : 'a . 'a Compare.comparaison -> ('a, unit) set -> ('a, unit) set =
+let right :
+  'a 'b . 'a Compare.comparaison -> ('a, 'b, unit) set -> ('a, 'b, unit) set
+  =
   fun f ->
     fun input -> match input with | Node (uu___, uu___1, uu___2, r) -> r
 let (max : Prims.int -> Prims.int -> Prims.int) =
   fun x -> fun y -> if x > y then x else y
-let rec member :
-  'a . 'a Compare.comparaison -> 'a -> ('a, unit) set -> Prims.bool =
-  fun f ->
-    fun x ->
-      fun input ->
-        match input with
-        | Leaf -> false
-        | Node (l, k, uu___, r) ->
-            ((Compare.uu___is_EQ (f x k)) || (member f x l)) ||
-              (member f x r)
+type ('a, 'b, 'f, 'x, 'input) member = Obj.t
 let delta :
-  'a .
-    'a Compare.comparaison -> ('a, unit) set -> ('a, unit) set -> Prims.nat
+  'a 'b .
+    'a Compare.comparaison ->
+      ('a, 'b, unit) set -> ('a, 'b, unit) set -> Prims.nat
   =
   fun f ->
     fun l ->
@@ -60,15 +67,15 @@ let delta :
         if (height f l) > (height f r)
         then (height f l) - (height f r)
         else (height f r) - (height f l)
-type ('a, 'f, 'input) is_avl = Obj.t
+type ('a, 'b, 'f, 'input) is_avl = Obj.t
 let make :
-  'a .
+  'a 'b .
     'a Compare.comparaison ->
-      ('a, unit) set -> 'a -> ('a, unit) set -> ('a, unit) set
+      ('a, 'b, unit) set ->
+        ('a * 'b) -> ('a, 'b, unit) set -> ('a, 'b, unit) set
   =
   fun f ->
     fun l ->
       fun k ->
         fun r ->
           Node (l, k, (Prims.int_one + (max (height f l) (height f r))), r)
-
