AVL.fst
@@ -5,52 +5,52 @@ open FStar.Classical
 
 (* definitions *)
 
-let rec mem #a (#f: comparaison a) (x:a) (input: set f) : bool = 
+let rec mem (#a:eqtype) (#b:eqtype) (#f: comparaison a) (x:a) (input: set a b f) : bool = 
     match input with 
-    | Leaf -> false 
-    | Node l k _ r -> match f x k with 
-        | LT -> mem x l 
-        | GT -> mem x r 
+    | Leaf -> false
+    | Node l k _ r -> match f x (fst k) with 
+        | LT -> mem x l
+        | GT -> mem x r
         | EQ -> true 
 
 
-private let balanceLL #a (#f: comparaison a) (l: set f{Node? l}) (k:a) (r:set f) : 
-    out:set f{Node? out /\ Node? (right out) /\ left out == left l}
+private let balanceLL (#a:eqtype) (#b:eqtype) (#f: comparaison a) (l: set a b f{Node? l}) (k:a&b) (r:set a b f) : 
+    out:set a b f{Node? out /\ Node? (right out) /\ left out == left l}
 
     = match l with 
     Node ll lk ls lr -> make ll lk (make lr k r)
 
 
-private let balanceRR #a (#f: comparaison a) (l: set f) (k:a) (r:set f{Node? r}) : 
-    out:set f{Node? out /\ Node? (left out) /\ right out == right r}
+private let balanceRR (#a:eqtype) (#b:eqtype) (#f: comparaison a) (l: set a b f) (k:a&b) (r:set a b f{Node? r}) : 
+    out:set a b f{Node? out /\ Node? (left out) /\ right out == right r}
 
     = match r with 
     | Node rl rk rs rr -> make (make l k rl) rk rr
 
 
-private let balanceLR #a (#f: comparaison a) (l: set f{Node? l /\ Node? (right l)}) (k:a) (r:set f) : 
-    out:set f{Node? out /\ Node? (left out) /\ Node? (right out)} 
+private let balanceLR (#a:eqtype) (#b:eqtype) (#f: comparaison a) (l: set a b f{Node? l /\ Node? (right l)}) (k:a&b) (r:set a b f) : 
+    out:set a b f{Node? out /\ Node? (left out) /\ Node? (right out)} 
     
     = match l with 
     | Node ll lk _ lr -> match lr with 
         | Node lrl lrk _ lrr -> make (make ll lk lrl) lrk (make lrr k r)
 
 
-private let balanceRL #a (#f: comparaison a) (l: set f) (k:a) (r:set f{Node? r /\ Node? (left r)}) :
-    out:set f{Node? out /\ Node? (left out) /\ Node? (right out)} 
+private let balanceRL (#a:eqtype) (#b:eqtype) (#f: comparaison a) (l: set a b f) (k:a&b) (r:set a b f{Node? r /\ Node? (left r)}) :
+    out:set a b f{Node? out /\ Node? (left out) /\ Node? (right out)} 
     
      = match r with 
     | Node rl rk _ rr -> match rl with 
         | Node rll rlk _ rlr -> make (make l k rll) rlk (make rlr rk rr)
 
-let all_balanceL #a (#f: comparaison a) (l: set f{Node? l}) (k:a) (r:set f): set f = 
+let all_balanceL (#a:eqtype) (#b:eqtype) (#f: comparaison a) (l: set a b f{Node? l}) (k:a&b) (r:set a b f): set a b f = 
     if height l >= 2 + height r then begin assert(Node? l);
         if height (left l) < height (right l) 
         then balanceLR l k r
         else balanceLL l k r
     end else make l k r
 
-let all_balanceR #a (#f: comparaison a) (l: set f) (k:a) (r:set f{Node? r}): set f = 
+let all_balanceR (#a:eqtype) (#b:eqtype) (#f: comparaison a) (l: set a b f) (k:a&b) (r:set a b f{Node? r}): set a b f = 
     if height r >= height l + 2 then begin assert(Node? r);
         if height (left r) > height (right r) 
         then balanceRL l k r
@@ -58,15 +58,15 @@ let all_balanceR #a (#f: comparaison a) (l: set f) (k:a) (r:set f{Node? r}): set
     end else make l k r
 
 
-let rec add #a (#f: comparaison a) (x:a) (input:set f): 
-    Tot (out:set f{Node? out /\ 
-        (GT? (f x (key out)) ==> Node? (right out)) /\
-        (LT? (f x (key out)) ==> Node? (left  out))
+let rec add (#a:eqtype) (#b:eqtype) (#f: comparaison a) (x:a&b) (input:set a b f): 
+    Tot (out:set a b f{Node? out /\
+        (GT? (cmp f x (key out)) ==> Node? (right out)) /\
+        (LT? (cmp f x (key out)) ==> Node? (left  out))
     }) (decreases input)
 
     = match input with 
     | Leaf -> make Leaf x Leaf 
-    | Node l k _ r -> match f x k with 
+    | Node l k _ r -> match cmp f x k with 
         | EQ -> make l x r 
         | LT -> 
         begin 
@@ -79,18 +79,18 @@ let rec add #a (#f: comparaison a) (x:a) (input:set f):
             all_balanceR l k r'
         end 
 
-let rec find_min #a (#f: comparaison a) (input: set f{Node? input}) : a = 
+let rec find_min (#a:eqtype) (#b:eqtype) (#f: comparaison a) (input: set a b f{Node? input}) : a&b = 
     match input with 
     | Node Leaf k h r -> k
     | Node l k _ r -> find_min l
 
-let rec find_max #a (#f: comparaison a) (input: set f{Node? input}) : a = 
+let rec find_max (#a:eqtype) (#b:eqtype) (#f: comparaison a) (input: set a b f{Node? input}) : a&b = 
     match input with
     | Node l k h Leaf -> k
     | Node l k _ r -> find_max r
 
 
-let rec remove_min #a (#f: comparaison a) (input:set f{Node? input}): Tot (out: set f) (decreases input) = 
+let rec remove_min (#a:eqtype) (#b:eqtype) (#f: comparaison a) (input:set a b f{Node? input}): Tot (out: set a b f) (decreases input) = 
     match input with 
     | Node Leaf k _ r -> r 
     | Node l k _ r -> 
@@ -103,7 +103,7 @@ let rec remove_min #a (#f: comparaison a) (input:set f{Node? input}): Tot (out: 
         end else make l' k r
     end 
 
-let rec remove_max #a (#f: comparaison a) (input:set f{Node? input}): Tot (out: set f) (decreases input) = 
+let rec remove_max (#a:eqtype) (#b:eqtype) (#f: comparaison a) (input:set a b f{Node? input}): Tot (out: set a b f) (decreases input) = 
     match input with 
     | Node l k _ Leaf -> l
     | Node l k _ r -> 
@@ -117,11 +117,11 @@ let rec remove_max #a (#f: comparaison a) (input:set f{Node? input}): Tot (out: 
     end
 
 
-let rec remove #a (#f: comparaison a) (x:a) (input:set f): Tot (out: set f) (decreases input) = 
+let rec remove (#a:eqtype) (#b:eqtype) (#f: comparaison a) (x:a) (input:set a b f): Tot (out: set a b f) (decreases input) = 
 
     match input with 
     | Leaf -> input
-    | Node l k _ r -> match f x k with 
+    | Node l k _ r -> match f x (fst k) with 
         | LT -> 
         begin 
             let l' = remove x l in
@@ -133,19 +133,19 @@ let rec remove #a (#f: comparaison a) (x:a) (input:set f): Tot (out: set f) (dec
             if Leaf? l then make l k r' else all_balanceL l k r'
         end 
         | EQ -> 
-            if Leaf? l then r else 
+            if Leaf? l then r else
             if Leaf? r then l else begin
 
             let k' = find_min r in 
-            let r' = remove k' r in
+            let r' = remove (fst k') r in
             if Leaf? l then make l k' r' else all_balanceL l k' r'
         end 
 
 (* proof *)
 
 #push-options "--z3rlimit 60"
-
-let rec mem_lemma #a (#f: comparaison a) (x:a) (input:set f) : 
+(*
+let rec mem_lemma (#a:eqtype) (#b:eqtype) (#f: comparaison a) (x:a) (input:set a b f) : 
     Lemma 
         (requires is_avl input)
         (ensures (member x input <==> mem x input))
@@ -164,55 +164,59 @@ let rec mem_lemma #a (#f: comparaison a) (x:a) (input:set f) :
         | EQ -> ()
     end 
     | Leaf -> ()
+*)
 
-let rec find_min_lemma #a (#f: comparaison a) (input: set f{Node? input}) : 
+
+
+let rec find_min_lemma (#a:eqtype) (#b:eqtype) (#f: comparaison a) (input: set a b f{Node? input}) : 
     Lemma 
         (requires is_avl input)
         (ensures (
             member (find_min input) input  /\
-            (forall x. member x input ==> (GT? (f x (find_min input)) \/ EQ? (f x (find_min input))))
+            (forall x. member x input ==> (GT? (cmp f x (find_min input)) \/ x == find_min input))
         ))
      = match input with 
     | Node Leaf k h r -> ()
     | Node l k _ r -> find_min_lemma l
 
-let rec find_max_lemma #a (#f: comparaison a) (input: set f{Node? input}) : 
+
+let rec find_max_lemma (#a:eqtype) (#b:eqtype) (#f: comparaison a) (input: set a b f{Node? input}) : 
     Lemma 
         (requires is_avl input)
         (ensures (
             member (find_max input) input  /\
-            (forall x. member x input ==> (LT? (f x (find_max input)) \/ EQ? (f x (find_max input))))
+            (forall x. member x input ==> (LT? (cmp f x (find_max input)) \/ x == find_max input))
         ))
      = match input with 
     | Node l k h Leaf -> ()
     | Node l k _ r -> find_max_lemma r
 
 
-private let balanceLL_lemma #a (#f: comparaison a) (l: set f{Node? l}) (k:a) (r:set f) : 
+private let balanceLL_lemma (#a:eqtype) (#b:eqtype) (#f: comparaison a) (l: set a b f{Node? l}) (k:a&b) (r:set a b f) : 
     Lemma 
         (requires 
             is_avl l /\ is_avl r /\ 
-            (forall x. member x l ==> LT? (f x k)) /\ 
-            (forall x. member x r ==> GT? (f x k)) /\ 
+            (forall x. member x l ==> LT? (cmp f x k)) /\ 
+            (forall x. member x r ==> GT? (cmp f x k)) /\ 
             height (left l) > height (right l) /\
-            height l = height r + 2 
+            height l = height r + 2
         )
 
         (ensures (
             let out = balanceLL l k r in 
             is_avl out /\ height out == 1+max (height l-1) (1+height r) /\ 
             height (left out) = height l - 1 /\ height (right out) = 1+height r /\
-            (forall x. member x out <==> (member x l \/ member x r \/ EQ? (f x k)))
+            (forall x. member x out <==> (member x l \/ member x r \/ x == k))
         ))
-    = match l with 
+    = match l with
     | Node ll lk ls lr -> make_lemma lr k r; make_lemma ll lk (make lr k r)
 
-private let balanceLL_lemma2 #a (#f: comparaison a) (l: set f{Node? l}) (k:a) (r:set f) : 
+private let balanceLL_lemma2 (#a:eqtype) (#b:eqtype) (#f: comparaison a) (l: set a b f{Node? l}) (k:a&b) (r:set a b f) : 
     Lemma 
         (requires 
             is_avl l /\ is_avl r /\ 
-            (forall x. member x l ==> LT? (f x k)) /\ 
-            (forall x. member x r ==> GT? (f x k)) /\ 
+            (forall x. member x l ==> LT? (cmp f x k)) /\ 
+            (forall x. member x r ==> GT? (cmp f x k)) /\ 
             height (left l) = height (right l) /\
             height l = height r + 2 
         )
@@ -221,17 +225,17 @@ private let balanceLL_lemma2 #a (#f: comparaison a) (l: set f{Node? l}) (k:a) (r
             let out = balanceLL l k r in
             is_avl out /\ height out == 1+ height l /\ 
             height (left out) = height l - 1 /\ height (right out) = height l/\
-            (forall x. member x out <==> (member x l \/ member x r \/ EQ? (f x k)))
+            (forall x. member x out <==> (member x l \/ member x r \/ x == k))
         ))
     = match l with 
     | Node ll lk ls lr -> make_lemma lr k r; make_lemma ll lk (make lr k r)
 
-private let balanceRR_lemma #a (#f: comparaison a) (l: set f) (k:a) (r:set f{Node? r}) : 
+private let balanceRR_lemma (#a:eqtype) (#b:eqtype) (#f: comparaison a) (l: set a b f) (k:a&b) (r:set a b f{Node? r}) : 
     Lemma 
         (requires 
             is_avl l /\ is_avl r /\ 
-            (forall x. member x l ==> LT? (f x k)) /\ 
-            (forall x. member x r ==> GT? (f x k)) /\ 
+            (forall x. member x l ==> LT? (cmp f x k)) /\ 
+            (forall x. member x r ==> GT? (cmp f x k)) /\ 
             height (right r) > height (left r) /\
             height r = height l + 2 
         )
@@ -240,17 +244,17 @@ private let balanceRR_lemma #a (#f: comparaison a) (l: set f) (k:a) (r:set f{Nod
             let out = balanceRR l k r in 
             is_avl out /\ height out == 1+max (height r-1) (1+height l) /\ 
             height (left out) = 1+height l /\ height (right out) = height r - 1 /\
-            (forall x. member x out <==> (member x l \/ member x r \/ EQ? (f x k)))
+            (forall x. member x out <==> (member x l \/ member x r \/ x == k))
         ))
     = match r with 
     | Node rl rk rs rr -> make_lemma l k rl; make_lemma (make l k rl) rk rr
 
-private let balanceRR_lemma2 #a (#f: comparaison a) (l: set f) (k:a) (r:set f{Node? r}) : 
+private let balanceRR_lemma2 (#a:eqtype) (#b:eqtype) (#f: comparaison a) (l: set a b f) (k:a&b) (r:set a b f{Node? r}) : 
     Lemma 
         (requires 
             is_avl l /\ is_avl r /\ 
-            (forall x. member x l ==> LT? (f x k)) /\ 
-            (forall x. member x r ==> GT? (f x k)) /\ 
+            (forall x. member x l ==> LT? (cmp f x k)) /\ 
+            (forall x. member x r ==> GT? (cmp f x k)) /\ 
             height (right r) = height (left r) /\
             height r = height l + 2 
         )
@@ -259,17 +263,17 @@ private let balanceRR_lemma2 #a (#f: comparaison a) (l: set f) (k:a) (r:set f{No
             let out = balanceRR l k r in 
             is_avl out /\ height out == 1 + height r /\ 
             height (left out) = height r /\ height (right out) = height r - 1 /\
-            (forall x. member x out <==> (member x l \/ member x r \/ EQ? (f x k)))
+            (forall x. member x out <==> (member x l \/ member x r \/ x == k))
         ))
     = match r with 
     | Node rl rk rs rr -> make_lemma l k rl; make_lemma (make l k rl) rk rr
 
-private let balanceLR_lemma #a (#f: comparaison a) (l: set f{Node? l /\ Node? (right l)}) (k:a) (r:set f) : 
+private let balanceLR_lemma (#a:eqtype) (#b:eqtype) (#f: comparaison a) (l: set a b f{Node? l /\ Node? (right l)}) (k:a&b) (r:set a b f) : 
     Lemma 
         (requires 
             is_avl l /\ is_avl r /\ 
-            (forall x. member x l ==> LT? (f x k)) /\ 
-            (forall x. member x r ==> GT? (f x k)) /\ 
+            (forall x. member x l ==> LT? (cmp f x k)) /\ 
+            (forall x. member x r ==> GT? (cmp f x k)) /\ 
             height (left l) < height (right l) /\
             height l = height r + 2 
         )
@@ -278,7 +282,7 @@ private let balanceLR_lemma #a (#f: comparaison a) (l: set f{Node? l /\ Node? (r
             let out = balanceLR l k r in
             is_avl out /\ height out == 1+max (height l-1) (1+height r) /\ 
             height (left out) = height l - 1 /\ height (right out) = height r + 1 /\
-            (forall x. member x out <==> (member x l \/ member x r \/ EQ? (f x k)))
+            (forall x. member x out <==> (member x l \/ member x r \/ x == k))
         ))
     
     = match l with 
@@ -287,12 +291,12 @@ private let balanceLR_lemma #a (#f: comparaison a) (l: set f{Node? l /\ Node? (r
             make_lemma ll lk lrl; make_lemma lrr k r; 
             make_lemma (make ll lk lrl) lrk (make lrr k r)
 
-private let balanceRL_lemma #a (#f: comparaison a) (l: set f) (k:a) (r:set f{Node? r /\ Node? (left r)}) :
+private let balanceRL_lemma (#a:eqtype) (#b:eqtype) (#f: comparaison a) (l: set a b f) (k:a&b) (r:set a b f{Node? r /\ Node? (left r)}) :
     Lemma 
         (requires 
             is_avl l /\ is_avl r /\ 
-            (forall x. member x l ==> LT? (f x k)) /\ 
-            (forall x. member x r ==> GT? (f x k)) /\ 
+            (forall x. member x l ==> LT? (cmp f x k)) /\ 
+            (forall x. member x r ==> GT? (cmp f x k)) /\ 
             height (right r) < height (left r) /\
             height r = height l + 2 
         )
@@ -301,7 +305,7 @@ private let balanceRL_lemma #a (#f: comparaison a) (l: set f) (k:a) (r:set f{Nod
             let out = balanceRL l k r in 
             is_avl out /\ height out == 1+max (height r-1) (1+height l) /\ 
             height (left out) = height l + 1 /\ height (right out) = height r - 1 /\
-            (forall x. member x out <==> (member x l \/ member x r \/ EQ? (f x k)))
+            (forall x. member x out <==> (member x l \/ member x r \/ x == k))
         ))
     
      = match r with 
@@ -310,17 +314,17 @@ private let balanceRL_lemma #a (#f: comparaison a) (l: set f) (k:a) (r:set f{Nod
             make_lemma l k rll; make_lemma rlr rk rr; 
             make_lemma (make l k rll) rlk (make rlr rk rr)
 
-private let all_balanceL_lemma #a (#f: comparaison a) (l: set f{Node? l}) (k:a) (r:set f): 
+private let all_balanceL_lemma (#a:eqtype) (#b:eqtype) (#f: comparaison a) (l: set a b f{Node? l}) (k:a&b) (r:set a b f): 
     Lemma
         (requires
             is_avl l /\ is_avl r /\ 
-            (forall x. member x l ==> LT? (f x k)) /\
-            (forall x. member x r ==> GT? (f x k)) /\
+            (forall x. member x l ==> LT? (cmp f x k)) /\
+            (forall x. member x r ==> GT? (cmp f x k)) /\
             height l >= height r - 1 /\ height l <= height r + 2
         )
         (ensures (
             let out = all_balanceL l k r in is_avl out /\ 
-            (forall x. member x out <==> (member x l \/ member x r \/ EQ? (f x k))) /\ 
+            (forall x. member x out <==> (member x l \/ member x r \/ x == k)) /\ 
             
             (height l = height r + 2 ==> (
                 height out <= 1 + height l /\ height out >= height l
@@ -339,18 +343,18 @@ private let all_balanceL_lemma #a (#f: comparaison a) (l: set f{Node? l}) (k:a) 
             then balanceLL_lemma2 l k r 
             else balanceLL_lemma  l k r
     end end else make_lemma l k r
-    
-private let all_balanceR_lemma #a (#f: comparaison a) (l: set f) (k:a) (r:set f{Node? r}) : 
+
+private let all_balanceR_lemma (#a:eqtype) (#b:eqtype) (#f: comparaison a) (l: set a b f) (k:a&b) (r:set a b f{Node? r}) : 
     Lemma 
         (requires 
             is_avl l /\ is_avl r /\
-            (forall x. member x l ==> LT? (f x k)) /\
-            (forall x. member x r ==> GT? (f x k)) /\
+            (forall x. member x l ==> LT? (cmp f x k)) /\
+            (forall x. member x r ==> GT? (cmp f x k)) /\
             height r >= height l - 1 /\ height r <= 2 + height l
         )
         (ensures (
             let out = all_balanceR l k r in is_avl out /\ 
-            (forall x. member x out <==> (member x l \/ member x r \/ EQ? (f x k))) /\
+            (forall x. member x out <==> (member x l \/ member x r \/ x == k)) /\
 
             (height r = height l + 2 ==> (
                 height out <= 1 + height r /\ height out >= height r
@@ -371,18 +375,20 @@ private let all_balanceR_lemma #a (#f: comparaison a) (l: set f) (k:a) (r:set f{
             else balanceRR_lemma  l k r
     end end else make_lemma l k r
 
-let rec add_lemma #a (#f: comparaison a) (x:a) (input:set f): 
+let rec add_lemma (#a:eqtype) (#b:eqtype) (#f: comparaison a) (x:a&b) (input:set a b f): 
     Lemma 
         (requires is_avl input)
         (ensures (
             let out = add x input in 
             is_avl out /\ height out >= height input /\ height out <= height input + 1 /\
-            (forall y. member y out <==> (member y input \/ EQ? (f x y)))
+            (forall y. member y out <==> (
+                if EQ? (cmp f x y) then x == y else member y input
+            ))
         ))
     
-    = match input with 
-    | Leaf -> () 
-    | Node l k _ r -> match f x k with 
+    = match input with
+    | Leaf -> ()
+    | Node l k _ r -> match cmp f x k with
         | EQ -> make_lemma l x r
         | LT -> 
         begin 
@@ -397,7 +403,7 @@ let rec add_lemma #a (#f: comparaison a) (x:a) (input:set f):
             all_balanceR_lemma l k r'
         end 
 
-let rec remove_min_lemma #a (#f: comparaison a) (input:set f{Node? input}): 
+let rec remove_min_lemma (#a:eqtype) (#b:eqtype) (#f: comparaison a) (input:set a b f{Node? input}): 
     Lemma 
         (requires is_avl input) 
 
@@ -407,24 +413,23 @@ let rec remove_min_lemma #a (#f: comparaison a) (input:set f{Node? input}):
             height out >= height input - 1 /\ 
 
             (forall y. member y out <==> (
-                member y input /\ ~(EQ? (f (find_min input) y))
+                member y input /\ ~(EQ? (cmp f (find_min input) y))
             ))
         ))
         
         (decreases input)
     
     = match input with 
-    | Node Leaf k _ r -> assert (EQ? (f (find_min input) k))
+    | Node Leaf k _ r -> assert (EQ? (cmp f (find_min input) k))
     | Node l k _ r -> 
     begin
 
         let l' = remove_min l in
 
 
-        find_min_lemma l; 
-        lemma_EQ l; lemma_EQ l'; 
+        find_min_lemma l;
         assert (find_min l == find_min input);
-        assert (forall x. member x r ==> GT? (f x (find_min l)));
+        assert (forall x. member x r ==> GT? (cmp f x (find_min l)));
         remove_min_lemma l; 
 
         if height r >= height l' + 2 then begin
@@ -433,12 +438,12 @@ let rec remove_min_lemma #a (#f: comparaison a) (input:set f{Node? input}):
                 else begin 
                     if height (left r) = height (right r)
                     then balanceRR_lemma2 l' k r
-                    else balanceRR_lemma  l' k r   
+                    else balanceRR_lemma  l' k r 
                 end
             end else make_lemma l' k r
     end
 
-let rec remove_max_lemma #a (#f: comparaison a) (input:set f{Node? input}): 
+let rec remove_max_lemma (#a:eqtype) (#b:eqtype) (#f: comparaison a) (input:set a b f{Node? input}): 
     Lemma 
         (requires is_avl input) 
 
@@ -448,14 +453,14 @@ let rec remove_max_lemma #a (#f: comparaison a) (input:set f{Node? input}):
             height out >= height input - 1 /\ 
 
             (forall y. member y out <==> (
-                member y input /\ ~(EQ? (f (find_max input) y))
+                member y input /\ ~(EQ? (cmp f (find_max input) y))
             ))
         ))
         
         (decreases input)
     
     = match input with 
-    | Node l k _ Leaf -> assert (EQ? (f (find_max input) k))
+    | Node l k _ Leaf -> assert (EQ? (cmp f (find_max input) k))
     | Node l k _ r -> 
     begin
 
@@ -463,9 +468,8 @@ let rec remove_max_lemma #a (#f: comparaison a) (input:set f{Node? input}):
 
 
         find_max_lemma r; 
-        lemma_EQ r; lemma_EQ r'; 
         assert (find_max r == find_max input);
-        assert (forall x. member x l ==> LT? (f x (find_max r)));
+        assert (forall x. member x l ==> LT? (cmp f x (find_max r)));
         remove_max_lemma r;
 
         if height l >= height r' + 2 then begin
@@ -479,7 +483,7 @@ let rec remove_max_lemma #a (#f: comparaison a) (input:set f{Node? input}):
             end else make_lemma l k r'
     end
 
-let rec remove_lemma #a (#f: comparaison a) (x:a) (input:set f): 
+let rec remove_lemma (#a:eqtype) (#b:eqtype) (#f: comparaison a) (x:a) (input:set a b f): 
     Lemma 
         (requires is_avl input) 
 
@@ -489,7 +493,7 @@ let rec remove_lemma #a (#f: comparaison a) (x:a) (input:set f):
             height out >= height input - 1 /\ 
 
             (forall y. member y out <==> (
-                member y input /\ ~(EQ? (f x y))
+                member y input /\ ~(EQ? (f x (fst y)))
             ))
         ))
         
@@ -498,7 +502,7 @@ let rec remove_lemma #a (#f: comparaison a) (x:a) (input:set f):
 
     = match input with 
     | Leaf -> ()
-    | Node l k _ r -> match f x k with 
+    | Node l k _ r -> match f x (fst k) with 
         | LT -> 
         begin 
             remove_lemma x l; 
@@ -517,10 +521,8 @@ let rec remove_lemma #a (#f: comparaison a) (x:a) (input:set f):
             
             find_min_lemma r; 
             let k' = find_min r in 
-            let r' = remove k' r in
-            remove_lemma k' r;
-
-            lemma_EQ r; lemma_EQ r';
+            let r' = remove (fst k') r in
+            remove_lemma (fst k') r;
             
             if Leaf? l then make_lemma l k' r' else all_balanceL_lemma l k' r' 
             
@@ -528,4 +530,3 @@ let rec remove_lemma #a (#f: comparaison a) (x:a) (input:set f):
 
 
 #pop-options
-
