BinTree.fst
@@ -1,84 +1,78 @@
 module BinTree 
 
+open FStar.Pervasives.Native
 open FStar.Classical
 open Compare 
 
+let cmp (#a:eqtype) (#b:eqtype) (f: comparaison a) (x:a&b) (y:a&b) : ordering = f (fst x) (fst y)
 
-type set #a (compare: comparaison a) = 
-    | Node : left: set compare -> a -> nat -> set compare -> set compare
-    | Leaf : set compare
+noeq
+type set (a: eqtype) (b: eqtype) (compare: comparaison a) = 
+    | Node : set a b compare -> (a&b) -> nat -> set a b compare -> set a b compare
+    | Leaf : set a b compare
 
-let height #a (#f: comparaison a) (s: set f): nat = match s with 
-    | Node l k s r -> s 
-    | Leaf -> 0 
+let height (#a:eqtype) (#b:eqtype) (#f: comparaison a) (s: set a b f): nat = match s with 
+    | Node l k s r -> s
+    | Leaf -> 0
 
-let key #a (#f: comparaison a) (s: set f{Node? s}) = match s with 
+let key (#a:eqtype) (#b:eqtype) (#f: comparaison a) (s: set a b f{Node? s}) = match s with 
     | Node _ k _ _ -> k
 
 
-let left #a (#f: comparaison a) (input: set f {Node? input}) : set f = 
+let left (#a:eqtype) (#b:eqtype) (#f: comparaison a) (input: set a b f {Node? input}) : set a b f = 
     match input with Node l _ _ _ -> l 
 
 
-let right #a (#f: comparaison a) (input: set f {Node? input}) : set f = 
+let right (#a:eqtype) (#b:eqtype) (#f: comparaison a) (input: set a b f {Node? input}) : set a b f = 
     match input with Node _ _ _ r -> r 
 
 
 let max x y = if x > y then x else y
 
 
-let rec member #a (#f: comparaison a) (x:a) (input: set f) : Tot bool (decreases input) = 
+let rec member (#a:eqtype) (#b:eqtype) (#f: comparaison a) (x:a&b) (input: set a b f) : Tot prop (decreases input) = 
     match input with 
     | Leaf -> false 
     | Node l k _ r -> 
     begin 
-        EQ? (f x k) || member x l || member x r
+        x == k \/ member x l \/ member x r
     end
 
 
-
-let delta #a (#f: comparaison a) (l: set f) (r: set f): nat = 
+let delta (#a:eqtype) (#b:eqtype) (#f: comparaison a) (l: set a b f) (r: set a b f): nat = 
     if height l > height r 
     then height l - height r
     else height r - height l
 
 
-let rec is_avl #a (#f: comparaison a) (input: set f): prop = match input with 
+let rec is_avl (#a:eqtype) (#b:eqtype) (#f: comparaison a) (input: set a b f): prop = match input with 
     | Node l k s r -> 
         s = max (height l) (height r) + 1 /\ 
         delta l r < 2 /\ is_avl l /\ is_avl r /\ 
-        (forall x. member x l ==> LT? (f x k)) /\ 
-        (forall x. member x r ==> GT? (f x k)) 
+        (forall x. member x l ==> LT? (cmp f x k)) /\
+        (forall x. member x r ==> GT? (cmp f x k))
     | Leaf -> true
 
 
-let make #a (#f: comparaison a) (l: set f) k (r: set f) : 
-    out:set f{Node? out /\ left out == l /\ right out == r /\ key out == k /\ height out = 1 + max (height l) (height r)} 
+let make (#a:eqtype) (#b:eqtype) (#f: comparaison a) (l: set a b f) k (r: set a b f) : 
+    out:set a b f{Node? out /\ left out == l /\ right out == r /\ key out == k /\ height out = 1 + max (height l) (height r)} 
     
     = Node l k (1 + max (height l) (height r)) r
 
-let make_lemma #a (#f: comparaison a) (l: set f) k (r: set f) : 
+let make_lemma (#a:eqtype) (#b:eqtype) (#f: comparaison a) (l: set a b f) k (r: set a b f) : 
     Lemma 
         (requires 
             is_avl l /\ is_avl r /\ 
-            (forall x. member x l ==> LT? (f x k)) /\ 
-            (forall x. member x r ==> GT? (f x k)) /\ 
+            (forall x. member x l ==> LT? (cmp f x k)) /\
+            (forall x. member x r ==> GT? (cmp f x k)) /\
             delta l r <= 1
         )
         
         (ensures (let out = make l k r in 
             is_avl out /\ height out == 1+max (height l) (height r) /\ 
-            (forall x. member x out <==> (member x l \/ member x r \/ EQ? (f x k))) /\ 
+            (forall x. member x out <==> (member x l \/ member x r \/ x == k)) /\
             Node? out /\ left out == l /\ right out == r /\ key out == k /\ height out = 1 + max (height l) (height r)
         )) = 
     
     ()
 
-let rec lemma_EQ #a (#f: comparaison a) (input: set f) : 
-    Lemma 
-        (forall x y. EQ? (f x y) ==>
-            (member x input <==> member y input)
-        )
-    = match input with 
-    | Node l k _ r -> lemma_EQ l; lemma_EQ r
-    | Leaf -> ()
